\documentclass[letterpaper, reqno,11pt]{article}
\usepackage[margin=1.0in]{geometry}
\usepackage{color,latexsym,amsmath,amssymb,graphicx, float}
\usepackage{hyperref}

\hypersetup{
colorlinks=true,
linkcolor=magenta,
filecolor=magenta,
urlcolor=cyan,
}

\graphicspath{ {images/} }

\begin{document}
\pagenumbering{arabic}
\title{Math 305 Homework 2}
\date{24/01/22}
\author{Xander Naumenko}
\maketitle

\vskip 0.5cm

10pts each

\noindent
1. Find all values of the following equation

(a)$ z^3= i-1$

\[
i-1=\sqrt{2}e^{i\frac{3\pi}{4}}=(2^{\frac{1}{6}}e^{ni\frac{\pi}{4}}+i\frac{2k\pi}{3})^3, k\in \{0,1,2\} 
.\]

(b) $ z^5= \frac{ 2i}{ 1-\sqrt{3} i}$

\[
\frac{2i}{1-\sqrt{3} }=\frac{-2\sqrt{3} +2i}{4}=-\frac{1}{2}\sqrt{3} +\frac{1}{2}i=e^{i\frac{5\pi}{6}}=e^{i\left( \frac{\pi}{6}+2k\frac{\pi}{5} \right) }, k\in \{0, \ldots, 5\} 
.\]

(c) $ (z-i)^2= i$

\[
    (z-i)^2=i=e^{i\frac{\pi}{2}}\implies z-i = e^{i\frac{\pi}{4}+i \pi k}\implies z=e^{i\frac{\pi}{4}+i \pi k}+e^{i\frac{\pi}{2}}, k\in \{0, 1\} 
.\]

(d) $z^2 +2i z+1=0 $

\[
z^2+2iz-1=(z+i)^2=-2=2e^{i\pi}\implies z+i=\sqrt{2} e^{i\left( \frac{\pi}{2}+\pi k \right) }\implies z=\sqrt{2} e^{i\left( \frac{\pi}{2}+\pi k \right) }-i, k\in \{0, 1\} 
.\]


\medskip

\noindent
*2. Let $m$ and $n$ be positive integers that have no common factor and $z_0$ be a complex number. Let $ z_0^{\frac{1}{n}}$ denote the set of all complex numbers such that $ z^n=z_0$, i.e., $ z_0^{\frac{1}{n}}=\{ z \ | z^n=z_0\}$. Prove that the set of numbers $(z_0^{1/n})^m$ is the same as the set of numbers $ (z_0^m)^{1/n}$.  Use this result to find all values of $ (1-i)^{3/2}$. Here $ (z_0^{1/n})^m=\{ z^m \ | z^n= z_0 \}$.

\medskip

Hint: since $ m$ and $n$ have no common factor, for any integer $k$, we can write it as $ k= m k_1+ n k_2$ where $k_1, k_2$ are two integers.


*: An extra 10points will be awarded to Problem 2 if your answer is correct. 

\medskip

Assume that $z_0=re^{i\phi}$. Then we have that $z_0^{1 /n}=e^{i\left( \frac{\phi}{n}+\frac{2\pi k}{n} \right) }, k\in\mathbb{Z}$ and $A=\left( z_0^m \right)^{1 /n}=e^{i\left( \frac{\phi m}{n}+\frac{2\pi k_1}{n} \right) }, k_1\in\mathbb{Z}$. Taking the first term to the power of $m$ gives $B=\left( z_0^{1 /n}\right)^{m}=e^{i\left( \frac{\phi m}{n}+\frac{2\pi k_2 m}{n} \right) }, k_2\in\mathbb{Z}$. To prove that these are equivalent sets, we will show that $\forall a\in A, a\in B$ and that $\forall b\in B, b\in A$, which is enough to show set equality. 

Let $b\in B$. It can thus be written as  $b=e^{i\left( \frac{\phi}{n}+\frac{2\pi k_2 m}{n} \right) }$ for some $k_2\in\mathbb{Z}$. Let $ k_1=k_2m$. Then we have that 
\[
b=e^{i\left( \frac{\phi}{n}+\frac{2\pi k_2 m}{n} \right) }=e^{i\left( \frac{\phi}{n}+\frac{2\pi k_1}{n} \right) }\in A
,\]
meaning $B\subseteq A$. 

For the other direction, let $a\in A$. Then it can be written as $e^{i\left( \frac{\phi m}{n}+\frac{2\pi k_1}{n} \right) }$ for some $k_1\in\mathbb{Z}$. Using the hint (sorry for the awkward choice of variable names), there exist $x, y\in\mathbb{Z}$ such that $k_1=mx+ny$. Plugging this in, we get 
\[
a=e^{i\left( \frac{\phi}{n}+\frac{2\pi k_1}{n} \right) }=e^{i\left( \frac{\phi}{n}+\frac{2\pi (mx+ny)}{n} \right) }=e^{i\left( \frac{\phi}{n}+\frac{2\pi mx}{n}+2\pi y \right) }=e^{i\left( \frac{\phi}{n}+\frac{2\pi mx}{n} \right) }
.\]
Letting $k_2=x$ it is clear that $a\in B\implies A\subseteq B$. 

Since we have shown that $A\subseteq B$ and $B\subseteq A$, it must be the case that $A=B$ as required. $\square$

To find the values of $(1-i)^{3 /2}$ we can expand, which is justified since the we just found that the order doesn't matter: 

\[
    (1-i)^{3 /2)}\left( (1-i)^{1 /2} \right)^3=\left(\sqrt[4]{2} e^{i\left( \frac{7}{8}\pi+\pi k \right) }\right)^3, k\in \{0, 1\} =2^{\frac{3}{4}}e^{i\left( \frac{7}{8}\pi+\pi k \right) }, k\in \{0, 1\} 
.\]

\medskip

\noindent
3. Write the following functions in the form $w= u(x, y)+ i v(x, y)$.

(a) $ f(z)= \frac{z+i}{z+1}$

\[
f(z)=\frac{z+i}{z+1}=\frac{x+i(y+1)}{(x+1)+iy}=\frac{(x+i(y+1))(x+1-iy)}{(x+1)^2+y^2}
.\]

\[
=\frac{x^2+x+y^2+y+i((y+1)(x+1)-xy)}{(x+1)^2-y^2}=\frac{x^2+x+y^2+y}{(x+1)^2+y^2}+i \frac{x+y+1}{(x+1)^2+y^2}
.\]

(b) $ f(z)= \frac{ e^z}{ z}$

\[
f(z)=\frac{e^z}{z}=\frac{e^{x+iy}}{x+iy}=\frac{e^{x}}{x^2+y^2}\left( x\cos y+y\sin y \right)+i\frac{e^{x}}{x^2+y^2} \left( x\sin y-y\cos y \right) 
.\]

(c) $ f(z)= \frac{ z^2+3}{|z-1|^2} $

\[
f(z)=\frac{x^2-y^2+2ixy+3}{(x-1)^2+y^2}=\frac{x^2-y^2+3}{(x-1)^2+y^2}+i \frac{2xy}{(x-1)^2+y^2}
.\]

\medskip


\noindent
4. Describe the image of the following sets under the following maps

(a) $ f(z)= (1-i) z+5$ for $ S=\{ Re (z)>0\}$

The multiplication by $1-i$ rotates the original set by $-\frac{\pi}{2}$ and scales by a factor of $ \sqrt{2} $, then adding 5 shifts the set 5 unites in the real axis. Thus the final set is
\[
f(S)=\{w\mid Re(w)>5+Im(w)\} 
.\]

(b) $ f(z)= \frac{z-i}{z+i}$ for $ S= \{ |z|<3 \}$

Expanding $f$ out we get 
% \[
% f(z)=\frac{z-i}{z+i}=\frac{x+(y-1)i}{x+i(y+1)}=\frac{x^2+y^2-1+2iyx}{x^2-(y+1)^2}
% .\]

\[
w=f(z)=\frac{z-i}{z+i}\implies z(1-w)-i=iw\implies z=\frac{i(w+1)}{1-w}%=i \frac{(u+1)+iv}{(1-u)-iv}
\]
% \[
% z=\frac{-u^2+1-v^2+2iv}{(1-u)^2-v^2}
% .\]
\[
|z|=\frac{|w+1|}{|w-1|}=\sqrt{\frac{(u+1)^2+v^2}{(u-1)^2+v^2}} < 3
\]
\[
\implies (u+1)^2+v^2<9(u-1)^2+9v^2\implies 1<8u^2-20u+9+8v^2=8\left(u-\frac{5}{4}\right)^2-\frac{7}{2}+8v^2
\]
\[
\implies \frac{9}{2}<8\left(u-\frac{5}{4}\right)^2+8v^2
.\]

This is the equation of a circle of radius $\frac{9}{2}$, with an offset of $\frac{5}{4}$ in the real direction: 
\[
f(S)=\{w\mid \left|w-\frac{5}{4}\right|>\frac{9}{2}\} 
.\]

(c) $ f(z)= -2 z^5$ for $ S= \{ |z|<1, 0<Arg z<\frac{\pi}{2} \}$

The image is contained in the circle around the origin of radius $2$ because $|z|<1$ and $f$ only scales it by $2$. For the argument, consider that $arg(w)=5arg(z)$ spans the interval $[0, 2\pi]$ since $0<arg(z)< \frac{\pi}{2}$. Thus the image is all the points contained in the circle of radius 2 centered at the origin: 
\[
f(S)=\{w\mid |w|<2\} 
.\]

\medskip

\noindent
5. Describe the image of the following sets under the given map

(a) $S= \{ Re (z)=1\}$, $w=e^z$

Since $Re(z)=1$, it must be in the form $z=1+iy, y\in\mathbb{R}$. Thus we have that 
 \[
w=e^{1+iy}=e\cdot e^{iy}
\]
which is just the equation for a circle of radius $e$: 
 \[
f(S)=\{w\mid |w|=e\} 
.\]

(b) $ S= \{ 0 \leq Im (z) \leq \frac{\pi}{4} \}$, $w=e^z$

Since $0\leq Im(z)\leq \frac{\pi}{4}$, the output $w=e^{z}=e^{x+iy}=e^xe^{iy}$ is constrained to the outputs with argument $0\leq Arg(w)\leq \frac{\pi}{4}$. Since there is no restriction on $Re(z)$ it encompasses the entire quadrant, so
\[
f(S)=\{w\mid 0\leq Arg(w)\leq \frac{\pi}{4}\} 
.\]

(c) $S= \{ 0\leq Re(z) \leq 1, Im (z)=1 \}$, $ w=z^2$

Based on the restrictions to $z$ it must be in the form $z=x+i, 0\leq x\leq 1$. Thus we have that 
\[
w=z^2=(x+i)^2=x^2+2xi-1=(x^2-1)+2xi=u+iv
.\]
Using these definitions for $u,v$, we know that $u=x^2-1=\frac{v^2}{4}-1$. This is the equation for a parabola oriented along the real axis offset by along the real axis, with only the line segment corresponding to $0\leq x\leq 1\implies 0\leq v\leq 2$ included. 
\[
f(S)=\{w\mid Re(w)=\frac{Im(w)^2}{4}-1, 0\leq Im(w)\leq 2\} 
.\]

\medskip

\noindent
6. The Joukowski map is defined by
$$ w=f(z)= \frac{1}{2} (z+\frac{1}{z} )$$


Show that $J$ maps the circle $ S=\{ |z|=r_0\}$ $(r_0>0, r_0\not =1$) onto an ellipse  $\frac{x^2}{a^2}+\frac{y^2}{b^2}=1$ and the unit circle $ S=\{ |z|=1\}$ onto the real interval $ [-1,1]$.

Hint: use polar form of $z$.

\medskip

For the first part let $z=r_0e^{i\theta}$. Then we get that 
\[
f(z)=\frac{1}{2}\left( r_0e^{i\theta}+r_0^{-1}e^{-i\theta} \right) =\frac{r_0}{2}\left( (1+\frac{1}{r_0^2})\cos\theta+i(1-\frac{1}{r_0^2})\sin\theta \right)
\]
\[
 =\frac{1}{2}\left( (1+\frac{1}{r_0^2})x+i(1-\frac{1}{r_0^2})y\right)=u+iv
.\]
Using the fact that $x^2+y^2=r_0^2$, we get that 
\[
1=r_0^{-2}\left( 4\left( 1+\frac{1}{r_0^2} \right)^{-2}u^2+4\left( 1-\frac{1}{r_0^2} \right)^{-2}v^2  \right)
\]
\[
\implies 1=\frac{4u^2}{(r_0+r_0^{-1})^2}+\frac{4v^2}{(r_0-r_0^{-1})^2}
.\]
Thus the output is an ellipse of the form $1=\frac{u^2}{ a^2}+\frac{v^2}{b^2}$, with $a=\frac{r_0^2+r_0}{2r_0}$ and $b=\frac{r_0^2-r_0}{ 2r_0}$. 

For the unit circle, we can no longer divide out by $r_0$ as we did in the previous part. Since it's on the unit circle $z=e^{i\theta}$, which means that 
\[
w=\frac{1}{2}\left(z+\frac{1}{z}\right)=\frac{1}{2}\left( e^{i\theta}+e^{-i\theta} \right) =\frac{1}{2}(2\cos\theta)=\cos\theta
.\]
As $\theta$ ranges over $\mathbb{R}$, $\cos\theta$ goes over the interval $[-1, 1]$ as required. 

\medskip

\noindent
7. Prove that $ |e^{-z^4}|\leq 1$ for all $z$ with $ -\frac{\pi}{8} \leq Arg (z) \leq \frac{\pi}{8}$.

\medskip

Let $z=re^{i\theta}$ with $Arg(z)=\theta$ between $-\frac{\pi}{8}$ and $\frac{\pi}{8}$. Then we have that 
\[
\left|e^{-z^{4}}\right|=\left|e^{-r\cos(4\theta)-ir \sin(4\theta)}\right|=\left| e^{-r\cos(4\theta)} \right| 
.\]
From the way we defined it we know that $-\frac{\pi}{8}\leq\theta\leq\frac{\pi}{8}\implies -\frac{\pi}{2}\leq\theta\leq\frac{\pi}{2}$. Since $\cos\theta>0$ for all such $\theta$, we have that 
\[
\left| e^{-z^{4}} \right| =\left| e^{-r\cos(4\theta)} \right| \leq \left| e^{-r} \right|\leq 1
.\]

\medskip

\noindent
8. Show that the function $ f(z)= \bar{z}$ is continuous everywhere but not differentiable anywhere.

\medskip

Let $\epsilon>0$, and select $\delta=\epsilon$. Then $\forall z\in\mathbb{C}$ with $|z-w|<\delta$, we have that
\[
|f(z)-f(w)|=|\overline{z}-\overline{w}|=|\overline{z-w}|=|z-w|<\delta=\epsilon
.\]
By the definition of the limit this implies that  implies that  
\[
\lim_{z\to w}z=w
\]
for all $w$, i.e. $\overline{z}$ is continuous everywhere. 

To show it is not differentiable anywhere, consider the the two paths approaching any point $w$ from both the real direction and the imaginary direction. Then we get that 
\[
    \lim_{h \to 0} \frac{\overline{z+h}-\overline{z}}{h}=\lim_{h \to 0}\frac{\overline{h}}{h}=\lim_{h \to 0}\frac{h}{h}=1
.\]
On the other hand if you approach from the imaginary axis, you get
\[
\lim_{h \to 0} \frac{\overline{z+ih}-\overline{z}}{ih}=\lim_{h \to 0}\frac{\overline{ih}}{ih}=\lim_{h \to 0}-\frac{ih}{ih}=-1
.\]
Since the derivative doesn't agree depending on the different paths, it must be that the function is differentiable nowhere. 

\medskip

\noindent
9. Discuss the differentiability and analyticity of the following functions

(a) $(x+\frac{x}{x^2+y^2})+ i (y-\frac{y}{x^2+y^2})$

To be differentiable the function must satisfy the Cauchy-Riemann equations: 
\[
u_x=1+\frac{x^2+y^2-2x^2}{(x^2+y^2)^2}=1+\frac{1}{x^2+y^2}-\frac{2x^2}{(x^2+y^2)^2}
\]
\[
v_y=1+\frac{1}{x^2+y^2}-\frac{2y^2}{(x^2+y^2)^2}
\]
\[
u_y=\frac{-2xy}{(x^2+y^2)^2}=-v_x
.\]
As can be seen $u_y=-v_x$ for all $x, y$, and $u_x=v_y$ when $x^2=y^2\implies |x|=|y|$. Thus the function is differentiable on the lines $x=y$ and $x=-y$. However since these are only lines, there are no neighborhoods over which the function is  analytic so it is nowhere analytic. 

(b) $ |z|^2+ 2z$

Rewritting we get that $|z|^2+2z=z\overline{z}+2z$. The Cauch-Riemann equations are equivalent to having no derivative with respect to $\overline{z}$, in this case we have 
\[
    \frac{\partial }{\partial \overline{z}} \left( z\overline{z}+2z \right) =z
.\]

This is only equal to 0 when $z=0$, so the function is only differentiable at $z=0$. Similarly to before, since there is only one point at which it is differentiable it is nowhere analytic. 


\noindent
10. Let
$$ f(z) = \left\{\begin{array}{l}
 ( x^{4/3} y^{5/3} + i x^{5/3} y^{4/3})/(x^2+y^2),  \mbox{if} \ z \not =0 ;\\
 0 \ \mbox{if} \ z=0
 \end{array}
 \right.
 $$
 Show that the Cauchy-Riemann equations hold at $z=0$ but $ f$ is not differentiable at $z=0$.

Hint: consider the limit with $\Delta z= (1+i) h, h \to 0$.

\medskip

First we show the Cauchy Riemann equations (I assume we don't have show differentiability of $u$ and $v$): 
\[
u_x=\frac {\frac{4}{3}x^{1 /3}y^{5 /3}}{ (x^2+y^2)}+\frac{2x^{7 /3}y^{5 /3}}{(x^2+y^2)^2}
.\]
\[
v_y=\frac {\frac{4}{3}y^{1 /3}x^{5 /3}}{ (x^2+y^2)}+\frac{2y^{7 /3}x^{5 /3}}{(x^2+y^2)^2}
.\]
\[
u_y=\frac{\frac{5}{3}x^{4 /3}y^{2 /3}}{x^2+y^2}+\frac{2y^{8 /3}x^{4 /3}}{x^2+y^2}
.\]
\[
v_x=\frac{\frac{5}{3}y^{4 /3}x^{2 /3}}{x^2+y^2}+\frac{2x^{8 /3}y^{4 /3}}{x^2+y^2}
.\]
Note that at $z=0$, $u_x=u_y=0$ and $u_y=-u_x=0$, so the Cauchy Riemann equations are obeyed. However, as the hint suggested consider the limit of the derivative with $\Delta z=(1+i)h$ as $h$ goes to zero. 

\[
\lim_{h \to 0}\frac{f(z+(1+i)h)-f(z)}{(1+i)h}=\lim_{h \to 0}\frac{h^{4 /3}h^{5 /3}+ih^{5 /3}y^{4 /3}}{(h^2+h^2)(1+i)h}=\lim_{h \to 0}\frac{h^3+ih^3}{(h^3+h^3)(1+i)}=\frac{1}{2}
.\]

Now consider the limit as $h$ approaches from the real axis. Then we have that 

\[
\lim_{h \to 0}\frac{f(z+h)-f(z)}{h}=\lim_{h \to 0}\frac{0}{h^3}=0
.\]

The two limits disagree, so it must be the case that the function is not differentiable at $z=0$. 


\end{document}


